Newest generic sender and receiver, with uuids

abp/SenderAutomaton.thy
@@ -3,7 +3,7 @@
  * This file was generated from Sender.maa and will be overridden when changed. To change
  * permanently, consider changing the model itself.
  *
- * Generated on Sep 22, 2018 6:29:44 PM by isartransformer 1.0.0
+ * Generated on Sep 24, 2018 5:01:53 PM by isartransformer 1.0.0
  *)
 theory SenderAutomaton
   imports bundle.tsynBundle automat.dAutomaton
@@ -26,21 +26,22 @@ setup_lifting type_definition_cfun
 fun prepend :: "'a::type list \<Rightarrow> 'a \<Rightarrow> 'a list" where
 "prepend xs x = x#xs"
 
+
 section \<open>Datatype definition\<close>
 
-datatype senderMessage = SenderBool "bool" | SenderNat "nat" | SenderPair_SenderNat_SenderBool "(nat\<times>bool)"
+datatype ('e::countable) senderMessage = DoNotUse_2ab8d3f31b8b462b9c9e2aac99cd809b_SenderBool "bool" | DoNotUse_2ab8d3f31b8b462b9c9e2aac99cd809b_SenderE "'e" | DoNotUse_2ab8d3f31b8b462b9c9e2aac99cd809b_SenderPair_SenderE_SenderBool "('e\<times>bool)"
 
-instance senderMessage :: countable
+instance senderMessage :: (countable) countable
   apply(intro_classes)
   by(countable_datatype)
 
-instantiation senderMessage :: message
+instantiation senderMessage :: (countable) message
 begin
-  fun ctype_senderMessage :: "channel \<Rightarrow> senderMessage set" where
+  fun ctype_senderMessage :: "channel \<Rightarrow> ('e::countable) senderMessage set" where
   "ctype_senderMessage c = (
-    if c = \<C> ''as'' then range SenderBool else
-    if c = \<C> ''i'' then range SenderNat else
-    if c = \<C> ''ds'' then range SenderPair_SenderNat_SenderBool else
+    if c = \<C> ''DoNotUse_2ab8d3f31b8b462b9c9e2aac99cd809b_as'' then range DoNotUse_2ab8d3f31b8b462b9c9e2aac99cd809b_SenderBool else
+    if c = \<C> ''DoNotUse_2ab8d3f31b8b462b9c9e2aac99cd809b_i'' then range DoNotUse_2ab8d3f31b8b462b9c9e2aac99cd809b_SenderE else
+    if c = \<C> ''DoNotUse_2ab8d3f31b8b462b9c9e2aac99cd809b_ds'' then range DoNotUse_2ab8d3f31b8b462b9c9e2aac99cd809b_SenderPair_SenderE_SenderBool else
     undefined)"
   instance
     by(intro_classes)
@@ -49,22 +50,22 @@ end
 
 section \<open>Helpers to create a bundle from a single raw element\<close>
 
-lift_definition senderElem_raw_as :: "bool \<Rightarrow> senderMessage tsyn sbElem" is
-"\<lambda>x. [\<C> ''as'' \<mapsto> Msg (SenderBool x)]"
+lift_definition senderElem_raw_as :: "bool \<Rightarrow> ('e::countable) senderMessage tsyn sbElem" is
+"\<lambda>x. [\<C> ''DoNotUse_2ab8d3f31b8b462b9c9e2aac99cd809b_as'' \<mapsto> Msg (DoNotUse_2ab8d3f31b8b462b9c9e2aac99cd809b_SenderBool x)]"
   unfolding sbElemWell_def
   unfolding usclOkay_stream_def
   unfolding ctype_tsyn_def
   by simp
 
-lift_definition senderElem_raw_i :: "nat \<Rightarrow> senderMessage tsyn sbElem" is
-"\<lambda>x. [\<C> ''i'' \<mapsto> Msg (SenderNat x)]"
+lift_definition senderElem_raw_i :: "'e \<Rightarrow> ('e::countable) senderMessage tsyn sbElem" is
+"\<lambda>x. [\<C> ''DoNotUse_2ab8d3f31b8b462b9c9e2aac99cd809b_i'' \<mapsto> Msg (DoNotUse_2ab8d3f31b8b462b9c9e2aac99cd809b_SenderE x)]"
   unfolding sbElemWell_def
   unfolding usclOkay_stream_def
   unfolding ctype_tsyn_def
   by simp
 
-lift_definition senderElem_raw_ds :: "(nat\<times>bool) \<Rightarrow> senderMessage tsyn sbElem" is
-"\<lambda>x. [\<C> ''ds'' \<mapsto> Msg (SenderPair_SenderNat_SenderBool x)]"
+lift_definition senderElem_raw_ds :: "('e\<times>bool) \<Rightarrow> ('e::countable) senderMessage tsyn sbElem" is
+"\<lambda>x. [\<C> ''DoNotUse_2ab8d3f31b8b462b9c9e2aac99cd809b_ds'' \<mapsto> Msg (DoNotUse_2ab8d3f31b8b462b9c9e2aac99cd809b_SenderPair_SenderE_SenderBool x)]"
   unfolding sbElemWell_def
   unfolding usclOkay_stream_def
   unfolding ctype_tsyn_def
@@ -73,135 +74,135 @@ lift_definition senderElem_raw_ds :: "(nat\<times>bool) \<Rightarrow> senderMess
 
 section \<open>Helpers to create a bundle from a single tsyn element\<close>
 
-fun senderElem_as :: "bool tsyn \<Rightarrow> senderMessage tsyn sbElem" where
+fun senderElem_as :: "bool tsyn \<Rightarrow> ('e::countable) senderMessage tsyn sbElem" where
 "senderElem_as (Msg port_as) = senderElem_raw_as port_as" |
-"senderElem_as null = sbeNull {\<C> ''as''}"
+"senderElem_as null = sbeNull {\<C> ''DoNotUse_2ab8d3f31b8b462b9c9e2aac99cd809b_as''}"
 
 declare senderElem_as.simps[simp del]
 
-definition sender_as :: "bool tsyn \<Rightarrow> senderMessage tsyn SB" where
+definition sender_as :: "bool tsyn \<Rightarrow> ('e::countable) senderMessage tsyn SB" where
 "sender_as port_as = sbe2SB (senderElem_as port_as)"
 
-fun senderElem_i :: "nat tsyn \<Rightarrow> senderMessage tsyn sbElem" where
+fun senderElem_i :: "'e tsyn \<Rightarrow> ('e::countable) senderMessage tsyn sbElem" where
 "senderElem_i (Msg port_i) = senderElem_raw_i port_i" |
-"senderElem_i null = sbeNull {\<C> ''i''}"
+"senderElem_i null = sbeNull {\<C> ''DoNotUse_2ab8d3f31b8b462b9c9e2aac99cd809b_i''}"
 
 declare senderElem_i.simps[simp del]
 
-definition sender_i :: "nat tsyn \<Rightarrow> senderMessage tsyn SB" where
+definition sender_i :: "'e tsyn \<Rightarrow> ('e::countable) senderMessage tsyn SB" where
 "sender_i port_i = sbe2SB (senderElem_i port_i)"
 
-fun senderElem_ds :: "(nat\<times>bool) tsyn \<Rightarrow> senderMessage tsyn sbElem" where
+fun senderElem_ds :: "('e\<times>bool) tsyn \<Rightarrow> ('e::countable) senderMessage tsyn sbElem" where
 "senderElem_ds (Msg port_ds) = senderElem_raw_ds port_ds" |
-"senderElem_ds null = sbeNull {\<C> ''ds''}"
+"senderElem_ds null = sbeNull {\<C> ''DoNotUse_2ab8d3f31b8b462b9c9e2aac99cd809b_ds''}"
 
 declare senderElem_ds.simps[simp del]
 
-definition sender_ds :: "(nat\<times>bool) tsyn \<Rightarrow> senderMessage tsyn SB" where
+definition sender_ds :: "('e\<times>bool) tsyn \<Rightarrow> ('e::countable) senderMessage tsyn SB" where
 "sender_ds port_ds = sbe2SB (senderElem_ds port_ds)"
 
 (* Create one sbElem for all input channels *)
-definition senderElemIn_as_i :: "bool tsyn \<Rightarrow> nat tsyn \<Rightarrow> senderMessage tsyn sbElem" where
+definition senderElemIn_as_i :: "bool tsyn \<Rightarrow> 'e tsyn \<Rightarrow> ('e::countable) senderMessage tsyn sbElem" where
 "senderElemIn_as_i port_as port_i = (senderElem_as port_as) \<plusminus> (senderElem_i port_i)"
 
 (* Create one sbElem for all output channels *)
-definition senderElemOut_ds :: "(nat\<times>bool) tsyn \<Rightarrow> senderMessage tsyn sbElem" where
+definition senderElemOut_ds :: "('e\<times>bool) tsyn \<Rightarrow> ('e::countable) senderMessage tsyn sbElem" where
 "senderElemOut_ds port_ds = (senderElem_ds port_ds)"
 
 (* Create one SB for all input channels *)
-definition senderIn_as_i :: "bool tsyn \<Rightarrow> nat tsyn \<Rightarrow> senderMessage tsyn SB" where
+definition senderIn_as_i :: "bool tsyn \<Rightarrow> 'e tsyn \<Rightarrow> ('e::countable) senderMessage tsyn SB" where
 "senderIn_as_i port_as port_i = (sbe2SB (senderElemIn_as_i port_as port_i))"
 
 (* Create one SB for all output channels *)
-definition senderOut_ds :: "(nat\<times>bool) tsyn \<Rightarrow> senderMessage tsyn SB" where
+definition senderOut_ds :: "('e\<times>bool) tsyn \<Rightarrow> ('e::countable) senderMessage tsyn SB" where
 "senderOut_ds port_ds = (sbe2SB (senderElemOut_ds port_ds))"
 
 
 section \<open>Helpers to create a bundle from a tsyn list of elements\<close>
 
-fun sender_list_as :: "(bool tsyn) list \<Rightarrow> senderMessage tsyn SB" where
+fun sender_list_as :: "(bool tsyn) list \<Rightarrow> ('e::countable) senderMessage tsyn SB" where
 "sender_list_as (x#xs) = ubConcEq (sender_as x)\<cdot>(sender_list_as xs)" |
-"sender_list_as []     = ubLeast {\<C> ''as''}"
+"sender_list_as []     = ubLeast {\<C> ''DoNotUse_2ab8d3f31b8b462b9c9e2aac99cd809b_as''}"
 
-fun sender_list_i :: "(nat tsyn) list \<Rightarrow> senderMessage tsyn SB" where
+fun sender_list_i :: "('e tsyn) list \<Rightarrow> ('e::countable) senderMessage tsyn SB" where
 "sender_list_i (x#xs) = ubConcEq (sender_i x)\<cdot>(sender_list_i xs)" |
-"sender_list_i []     = ubLeast {\<C> ''i''}"
+"sender_list_i []     = ubLeast {\<C> ''DoNotUse_2ab8d3f31b8b462b9c9e2aac99cd809b_i''}"
 
-fun sender_list_ds :: "((nat\<times>bool) tsyn) list \<Rightarrow> senderMessage tsyn SB" where
+fun sender_list_ds :: "(('e\<times>bool) tsyn) list \<Rightarrow> ('e::countable) senderMessage tsyn SB" where
 "sender_list_ds (x#xs) = ubConcEq (sender_ds x)\<cdot>(sender_list_ds xs)" |
-"sender_list_ds []     = ubLeast {\<C> ''ds''}"
+"sender_list_ds []     = ubLeast {\<C> ''DoNotUse_2ab8d3f31b8b462b9c9e2aac99cd809b_ds''}"
 
 (* Create one SB for all input channels *)
-definition senderIn_list_as_i :: "bool tsyn list \<Rightarrow> nat tsyn list \<Rightarrow> senderMessage tsyn SB" where
+definition senderIn_list_as_i :: "bool tsyn list \<Rightarrow> 'e tsyn list \<Rightarrow> ('e::countable) senderMessage tsyn SB" where
 "senderIn_list_as_i port_as port_i = (sender_list_as port_as) \<uplus> (sender_list_i port_i)"
 
 (* Create one SB for all output channels *)
-definition senderOut_list_ds :: "(nat\<times>bool) tsyn list \<Rightarrow> senderMessage tsyn SB" where
+definition senderOut_list_ds :: "('e\<times>bool) tsyn list \<Rightarrow> ('e::countable) senderMessage tsyn SB" where
 "senderOut_list_ds port_ds = (sender_list_ds port_ds)"
 
 
 section \<open>Helpers to create a bundle from a tsyn stream of elements\<close>
 
-lift_definition sender_stream_as_h :: "bool tsyn stream \<Rightarrow> senderMessage tsyn SB" is
-"\<lambda> s. [(\<C> ''as'') \<mapsto> (tsynMap (SenderBool)\<cdot>s)]"
+lift_definition DoNotUse_2ab8d3f31b8b462b9c9e2aac99cd809b_sender_stream_as_h :: "bool tsyn stream \<Rightarrow> ('e::countable) senderMessage tsyn SB" is
+"\<lambda> s. [(\<C> ''DoNotUse_2ab8d3f31b8b462b9c9e2aac99cd809b_as'') \<mapsto> (tsynMap (DoNotUse_2ab8d3f31b8b462b9c9e2aac99cd809b_SenderBool)\<cdot>s)]"
   unfolding ubWell_def usclOkay_stream_def ctype_tsyn_def
   apply auto
   sorry
 
-lift_definition sender_stream_as :: "(bool) tsyn stream \<rightarrow> senderMessage tsyn SB" is
-"sender_stream_as_h"
+lift_definition sender_stream_as :: "(bool) tsyn stream \<rightarrow> ('e::countable) senderMessage tsyn SB" is
+"DoNotUse_2ab8d3f31b8b462b9c9e2aac99cd809b_sender_stream_as_h"
   sorry
 
-lift_definition sender_stream_i_h :: "nat tsyn stream \<Rightarrow> senderMessage tsyn SB" is
-"\<lambda> s. [(\<C> ''i'') \<mapsto> (tsynMap (SenderNat)\<cdot>s)]"
+lift_definition DoNotUse_2ab8d3f31b8b462b9c9e2aac99cd809b_sender_stream_i_h :: "'e tsyn stream \<Rightarrow> ('e::countable) senderMessage tsyn SB" is
+"\<lambda> s. [(\<C> ''DoNotUse_2ab8d3f31b8b462b9c9e2aac99cd809b_i'') \<mapsto> (tsynMap (DoNotUse_2ab8d3f31b8b462b9c9e2aac99cd809b_SenderE)\<cdot>s)]"
   unfolding ubWell_def usclOkay_stream_def ctype_tsyn_def
   apply auto
   sorry
 
-lift_definition sender_stream_i :: "(nat) tsyn stream \<rightarrow> senderMessage tsyn SB" is
-"sender_stream_i_h"
+lift_definition sender_stream_i :: "('e) tsyn stream \<rightarrow> ('e::countable) senderMessage tsyn SB" is
+"DoNotUse_2ab8d3f31b8b462b9c9e2aac99cd809b_sender_stream_i_h"
   sorry
 
-lift_definition sender_stream_ds_h :: "(nat\<times>bool) tsyn stream \<Rightarrow> senderMessage tsyn SB" is
-"\<lambda> s. [(\<C> ''ds'') \<mapsto> (tsynMap (SenderPair_SenderNat_SenderBool)\<cdot>s)]"
+lift_definition DoNotUse_2ab8d3f31b8b462b9c9e2aac99cd809b_sender_stream_ds_h :: "('e\<times>bool) tsyn stream \<Rightarrow> ('e::countable) senderMessage tsyn SB" is
+"\<lambda> s. [(\<C> ''DoNotUse_2ab8d3f31b8b462b9c9e2aac99cd809b_ds'') \<mapsto> (tsynMap (DoNotUse_2ab8d3f31b8b462b9c9e2aac99cd809b_SenderPair_SenderE_SenderBool)\<cdot>s)]"
   unfolding ubWell_def usclOkay_stream_def ctype_tsyn_def
   apply auto
   sorry
 
-lift_definition sender_stream_ds :: "((nat\<times>bool)) tsyn stream \<rightarrow> senderMessage tsyn SB" is
-"sender_stream_ds_h"
+lift_definition sender_stream_ds :: "(('e\<times>bool)) tsyn stream \<rightarrow> ('e::countable) senderMessage tsyn SB" is
+"DoNotUse_2ab8d3f31b8b462b9c9e2aac99cd809b_sender_stream_ds_h"
   sorry
 
 (* Create one SB for all input channels *)
-definition senderIn_stream_as_i :: "bool tsyn stream \<rightarrow> nat tsyn stream \<rightarrow> senderMessage tsyn SB" where
+definition senderIn_stream_as_i :: "bool tsyn stream \<rightarrow> 'e tsyn stream \<rightarrow> ('e::countable) senderMessage tsyn SB" where
 "senderIn_stream_as_i = (\<Lambda>  port_as port_i. (sender_stream_as\<cdot>port_as) \<uplus> (sender_stream_i\<cdot>port_i))"
 
 (* Create one SB for all output channels *)
-definition senderOut_stream_ds :: "(nat\<times>bool) tsyn stream \<rightarrow> senderMessage tsyn SB" where
+definition senderOut_stream_ds :: "('e\<times>bool) tsyn stream \<rightarrow> ('e::countable) senderMessage tsyn SB" where
 "senderOut_stream_ds = (\<Lambda>  port_ds. (sender_stream_ds\<cdot>port_ds))"
 
 
 section \<open>Helpers to get tsyn elements and streams from sbElems and SBs\<close>
 
-fun senderElem_get_as :: "senderMessage tsyn sbElem \<Rightarrow> (bool) tsyn" where
+fun senderElem_get_as :: "('e::countable) senderMessage tsyn sbElem \<Rightarrow> (bool) tsyn" where
 "senderElem_get_as sbe = undefined"
 
-lift_definition sender_get_stream_as :: "senderMessage tsyn SB \<rightarrow> bool tsyn stream" is
-"\<lambda>sb. tsynMap (inv SenderBool)\<cdot>(sb . (\<C> ''as''))"
+lift_definition sender_get_stream_as :: "('e::countable) senderMessage tsyn SB \<rightarrow> bool tsyn stream" is
+"\<lambda>sb. tsynMap (inv DoNotUse_2ab8d3f31b8b462b9c9e2aac99cd809b_SenderBool)\<cdot>(sb . (\<C> ''DoNotUse_2ab8d3f31b8b462b9c9e2aac99cd809b_as''))"
   by(simp add: cfun_def)
 
-fun senderElem_get_i :: "senderMessage tsyn sbElem \<Rightarrow> (nat) tsyn" where
+fun senderElem_get_i :: "('e::countable) senderMessage tsyn sbElem \<Rightarrow> ('e) tsyn" where
 "senderElem_get_i sbe = undefined"
 
-lift_definition sender_get_stream_i :: "senderMessage tsyn SB \<rightarrow> nat tsyn stream" is
-"\<lambda>sb. tsynMap (inv SenderNat)\<cdot>(sb . (\<C> ''i''))"
+lift_definition sender_get_stream_i :: "('e::countable) senderMessage tsyn SB \<rightarrow> 'e tsyn stream" is
+"\<lambda>sb. tsynMap (inv DoNotUse_2ab8d3f31b8b462b9c9e2aac99cd809b_SenderE)\<cdot>(sb . (\<C> ''DoNotUse_2ab8d3f31b8b462b9c9e2aac99cd809b_i''))"
   by(simp add: cfun_def)
 
-fun senderElem_get_ds :: "senderMessage tsyn sbElem \<Rightarrow> ((nat\<times>bool)) tsyn" where
+fun senderElem_get_ds :: "('e::countable) senderMessage tsyn sbElem \<Rightarrow> (('e\<times>bool)) tsyn" where
 "senderElem_get_ds sbe = undefined"
 
-lift_definition sender_get_stream_ds :: "senderMessage tsyn SB \<rightarrow> (nat\<times>bool) tsyn stream" is
-"\<lambda>sb. tsynMap (inv SenderPair_SenderNat_SenderBool)\<cdot>(sb . (\<C> ''ds''))"
+lift_definition sender_get_stream_ds :: "('e::countable) senderMessage tsyn SB \<rightarrow> ('e\<times>bool) tsyn stream" is
+"\<lambda>sb. tsynMap (inv DoNotUse_2ab8d3f31b8b462b9c9e2aac99cd809b_SenderPair_SenderE_SenderBool)\<cdot>(sb . (\<C> ''DoNotUse_2ab8d3f31b8b462b9c9e2aac99cd809b_ds''))"
   by(simp add: cfun_def)
 
 
@@ -212,22 +213,21 @@ section \<open>Automaton definition\<close>
 datatype SenderSubstate = Sf | St
 
 (* And these have also the variables *)
-datatype SenderState = SenderState SenderSubstate (* buffer = *) "nat list" (* c = *) "nat"
+datatype 'e SenderState = SenderState SenderSubstate (* buffer = *) "'e list" (* c = *) "nat"
 
 (* Function to get the substate *)
-fun getSenderSubState :: "SenderState \<Rightarrow> SenderSubstate" where
+fun getSenderSubState :: "'e SenderState \<Rightarrow> SenderSubstate" where
 "getSenderSubState (SenderState s _ _) = s"
 
 (* Functions to get the variables *)
-fun getBuffer :: "SenderState \<Rightarrow> nat list" where
+fun getBuffer :: "'e SenderState \<Rightarrow> 'e list" where
 "getBuffer (SenderState _ var_buffer var_c) = var_buffer"
 
-fun getC :: "SenderState \<Rightarrow> nat" where
+fun getC :: "'e SenderState \<Rightarrow> nat" where
 "getC (SenderState _ var_buffer var_c) = var_c"
 
-
 (* Helper that allows us to utilize pattern matching *)
-fun senderTransitionH :: "(SenderState \<times> (bool tsyn \<times> nat tsyn)) \<Rightarrow> (SenderState \<times> senderMessage tsyn SB)" where
+fun senderTransitionH :: "('e SenderState \<times> (bool tsyn \<times> 'e tsyn)) \<Rightarrow> ('e SenderState \<times> ('e::countable) senderMessage tsyn SB)" where
 "senderTransitionH (SenderState Sf var_buffer var_c, (\<^cancel>\<open>as\<mapsto>\<close>Msg port_as, \<^cancel>\<open>i\<mapsto>\<close>Msg port_i)) =
   (if((size var_buffer)>1 \<and> port_as=False) then ((SenderState St (prepend (butlast var_buffer) port_i) 3, (senderOut_ds (Msg (Pair (last (butlast var_buffer)) True)))))
    else if((size var_buffer)=1 \<and> port_as=False) then ((SenderState St (prepend (butlast var_buffer) port_i) 3, (senderOut_ds (Msg (Pair port_i True)))))
@@ -286,36 +286,36 @@ fun senderTransitionH :: "(SenderState \<times> (bool tsyn \<times> nat tsyn)) \
 
 (* Domain *)
 definition senderDom :: "channel set" where
-"senderDom = {\<C> ''as'', \<C> ''i''}"
+"senderDom = {\<C> ''DoNotUse_2ab8d3f31b8b462b9c9e2aac99cd809b_as'', \<C> ''DoNotUse_2ab8d3f31b8b462b9c9e2aac99cd809b_i''}"
 
 (* Range *)
 definition senderRan :: "channel set" where
-"senderRan = {\<C> ''ds''}"
+"senderRan = {\<C> ''DoNotUse_2ab8d3f31b8b462b9c9e2aac99cd809b_ds''}"
 
 (* Transition function *)
-definition senderTransition :: "(SenderState \<times> senderMessage tsyn sbElem) \<Rightarrow> (SenderState \<times> senderMessage tsyn SB)" where
+definition senderTransition :: "('e SenderState \<times> ('e::countable) senderMessage tsyn sbElem) \<Rightarrow> ('e SenderState \<times> ('e::countable) senderMessage tsyn SB)" where
 "senderTransition = (\<lambda> (s,b). (if (sbeDom b) = senderDom then senderTransitionH (s, (senderElem_get_as b, senderElem_get_i b)) else undefined))"
 
 (* Initial state *)
-definition senderInitialState :: "SenderState" where
-"senderInitialState = SenderState St []  0"
+definition senderInitialState :: "'e SenderState" where
+"senderInitialState = SenderState St ([] ::'e list) (0::nat)"
 
 (* Initial output *)
-definition senderInitialOutput :: "senderMessage tsyn SB" where
+definition senderInitialOutput :: "('e::countable) senderMessage tsyn SB" where
 "senderInitialOutput = senderOut_ds null"
 
 (* The final automaton *)
-lift_definition senderAutomaton :: "(SenderState, senderMessage tsyn) dAutomaton" is
+lift_definition senderAutomaton :: "('e SenderState, ('e::countable) senderMessage tsyn) dAutomaton" is
 "(senderTransition, senderInitialState, senderInitialOutput, senderDom, senderRan)"
   by (simp add: senderDom_def senderRan_def)
 
 (* Stream processing function for each state (handy for step lemmata) *)
-definition senderStep :: "(SenderState \<Rightarrow> (senderMessage tsyn, senderMessage tsyn) SPF)" where
+definition senderStep :: "('e SenderState \<Rightarrow> (('e::countable) senderMessage tsyn, ('e::countable) senderMessage tsyn) SPF)" where
 "senderStep = da_h senderAutomaton"
 
 (* The final SPF *)
-definition senderSPF :: "(senderMessage tsyn, senderMessage tsyn) SPF" where
-"senderSPF = da_H senderAutomaton"
+definition senderSPF :: "(('e::countable) senderMessage tsyn, ('e::countable) senderMessage tsyn) SPF" where
+"senderSPF = da_H (senderAutomaton::('e SenderState, ('e::countable) senderMessage tsyn) dAutomaton)"
 
 
 section \<open>Lemmas for automaton definition\<close>
@@ -704,7 +704,7 @@ lemma senderTransition_7_2[simp]:
 section \<open>Step-wise lemmata for the SPF\<close>
 
 (* Convert the SPF to step notation *)
-lemma senderSpf2Step: "senderSPF = spfConcOut (senderOut_ds null)\<cdot>(senderStep (SenderState St []  0))"
+lemma senderSpf2Step: "senderSPF = spfConcOut (senderOut_ds null)\<cdot>(senderStep (SenderState St ([] ::'e::countable list) (0::nat)))"
   sorry
 
 (* Line 33:  Sf -> St [buffer.size()>1 && i!=null] {as==false} / {buffer=buffer.butlast().prepend(i), c=3, ds=new Pair<>(buffer.butlast().last(),true)}; *)
